\documentclass[12pt, a4paper]{report}

\usepackage{amsmath}
\usepackage{amssymb}
\usepackage{ragged2e}

\title{Esericitazione}
\author{Gabr1313}
\date{\today}


\begin{document}
\justify

\maketitle
\tableofcontents

\chapter{Esercitazione 1}

\section{Limiti}

\paragraph{Es}
\[
    \lim_{\rho \to 0} \frac{\rho (|\cos^2 \theta)| + |\cos^2 \theta \sin 
    \theta|)}{1} \leq \rho(1+1) = 2\rho = 0
\]
\paragraph{Es}
\[
    \lim_{(x,y) \to (2, -1)} \frac{(y^2 - x^2 + 3)^2}{(x - 2)^2  + (y + 1)^2} =
\]
\subparagraph{Primo modo} 
\begin{cases}
    $X = x-2$ \\
    $Y = y + 1$
\end{cases}
\subparagraph{Secondo modo} 
\begin{cases}
    $x = 2 + \roh \cos \theta$ \\
    $y = -1 + \roh \cos \theta$
\end{cases}
\[
    \lim_{\rho \to 0^+} \frac{((-1 + \roh \sin \theta)^2 - 
    (2 + \roh \cos\theta) ^2 + 3)^2}{\rho \cos^2 \theta + \rho^2 \sin^2 \theta}
    = \lim_{\rho \to 0^+} (\rho - 2 \sin \theta - \cos \theta)^2
    \Rightarrow \nexists
\]


\end{document}
